# Copyright (c) 2025 Robert Bosch Manufacturing Solutions GmbH
#
#  See the AUTHORS file(s) distributed with this work for additional
#  information regarding authorship.
#
#  This Source Code Form is subject to the terms of the Mozilla Public
#  License, v. 2.0. If a copy of the MPL was not distributed with this
#  file, You can obtain one at https://mozilla.org/MPL/2.0/.
#
# SPDX-License-Identifier: MPL-2.0

@prefix mmm: <urn:samm:org.eclipse.esmf.samm:meta-meta-model:2.3.0#> .
@prefix samm: <urn:samm:org.eclipse.esmf.samm:meta-model:2.3.0#> .
@prefix rdf: <http://www.w3.org/1999/02/22-rdf-syntax-ns#> .
@prefix rdfs: <http://www.w3.org/2000/01/rdf-schema#> .
@prefix xsd: <http://www.w3.org/2001/XMLSchema#> .

# Meta meta model concepts
mmm:Concept rdfs:subClassOf rdfs:Class .

mmm:NamedConcept rdfs:subClassOf mmm:Concept .

mmm:ConceptWithProperties rdfs:subClassOf mmm:Concept .

mmm:Attribute rdfs:subClassOf rdf:Property .

mmm:Constant rdfs:subClassOf rdfs:Resource .

mmm:PropertyUsage rdfs:subClassOf rdfs:Class .

# Meta model concepts
samm:Aspect rdfs:subClassOf mmm:NamedConcept, mmm:ConceptWithProperties ;
   rdfs:label "Aspect" ;
   rdfs:comment "An Aspect is the root element of each Aspect Model and has a number of Properties and Operations." .

samm:Entity rdfs:subClassOf mmm:NamedConcept, mmm:ConceptWithProperties ;
   rdfs:label "Entity" ;
   rdfs:comment "An Entity is a logical encapsulation of multiple values. It has a number of Properties." .

samm:AbstractEntity rdfs:subClassOf mmm:NamedConcept, mmm:ConceptWithProperties ;
   rdfs:label "AbstractEntity" ;
   rdfs:comment "An Abstract Entity is a logical encapsulation of a shared concept." .

samm:Property rdfs:subClassOf mmm:NamedConcept ;
   rdfs:label "Property" ;
   rdfs:comment "A Property represents a named value." .

samm:AbstractProperty rdfs:subClassOf mmm:NamedConcept ;
   rdfs:label "AbstractProperty" ;
   rdfs:comment "A Property that has no Characteristic set." .

samm:Characteristic rdfs:subClassOf mmm:Concept ;
   rdfs:label "Characteristic" ;
   rdfs:comment "A Characteristic describes a Property's meaning in the context of the Aspect." .

samm:Constraint rdfs:subClassOf mmm:Concept ;
   rdfs:label "Constraint" ;
   rdfs:comment "A Constraint can be used to further specify a Characteristic, for example on the value range." .

samm:Operation rdfs:subClassOf mmm:NamedConcept ;
   rdfs:label "Operation" ;
   rdfs:comment "An Operation represents an action that can be triggered on the device that is represented by the Digital Twin, for example switching a part of a machine on or off." .

samm:Event rdfs:subClassOf mmm:NamedConcept ;
   rdfs:label "Event" ;
   rdfs:comment "An Event is a model element that represents a single occurence where the timing is important. Assets can for instance emit events to notify other assets in case of special occurences." .

samm:Unit rdfs:subClassOf mmm:NamedConcept ;
   rdfs:label "Unit" ;
   rdfs:comment "A Unit refers to a physical unit, such as metre or degree celsius." .

samm:QuantityKind rdfs:subClassOf mmm:NamedConcept ;
   rdfs:label "QuantityKind" ;
   rdfs:comment "A Quantity Kind describes the kind a Unit refers to, such as length or temperature.".

samm:Namespace rdfs:subClassOf mmm:NamedConcept ;
   rdfs:label "Namespace" ;
   rdfs:comment "A Namespace can provide a human-readable name and a description for namespaces." .

samm:Value rdfs:subClassOf mmm:ConceptWithProperties ;
   rdfs:label: "Value" ;
   rdfs:comment "A type is designed to represent a value enriched with semantic metadata.".

# Meta meta model attributes used in Shapes
mmm:listType a rdf:Property ;
   rdfs:label "listType" ;
   rdfs:comment "Used to define the type for a list Property." ;
   rdfs:range rdfs:Resource .

# Meta model attributes
samm:preferredName a mmm:Attribute ;
   rdfs:label "preferredName" ;
   rdfs:comment "Human readable name in a specific language." ;
   rdfs:domain mmm:Concept ;
   rdfs:range rdf:langString .

samm:description a mmm:Attribute ;
   rdfs:label "description" ;
   rdfs:comment "Human readable description in a specific language" ;
   rdfs:domain mmm:Concept ;
   rdfs:range rdf:langString .

samm:dataType a mmm:Attribute ;
   rdfs:label "dataType" ;
   rdfs:comment "Reference to a scalar or complex (Entity) data type." ;
   rdfs:domain samm:Characteristic ;
   rdfs:range rdfs:Resource .

samm:value a mmm:Attribute ;
   rdfs:label "value" ;
   rdfs:comment "A single constant value or link to another resource." ;
   rdfs:domain mmm:Concept ;
   rdfs:range rdfs:Resource .

samm:properties a mmm:Attribute ;
   rdfs:label "properties" ;
   rdfs:comment "The list of Properties of an Aspect or Entity" ;
   rdfs:domain mmm:ConceptWithProperties ;
   rdfs:range rdfs:Resource .

samm:characteristic a mmm:Attribute ;
   rdfs:label "characteristic" ;
   rdfs:comment "The Characteristic describing a Property." ;
   rdfs:domain samm:Property ;
   rdfs:range rdfs:Resource .

samm:operations a mmm:Attribute ;
   rdfs:label "operations" ;
   rdfs:comment "The list of Operations of an Aspect." ;
   rdfs:domain samm:Aspect ;
   rdfs:range rdfs:Resource .

samm:input a mmm:Attribute ;
   rdfs:label "input" ;
   rdfs:comment "A list of references to Properties that describe the input to an operation." ;
   rdfs:domain samm:Operation ;
   rdfs:range rdfs:Resource .

samm:output a mmm:Attribute ;
   rdfs:label "output" ;
   rdfs:comment "A single reference to a Property that describes the output of an operation." ;
   rdfs:domain samm:Operation ;
   rdfs:range rdfs:Resource .

samm:events a mmm:Attribute ;
   rdfs:label "events" ;
   rdfs:comment "The list of Events of an Aspect." ;
   rdfs:domain samm:Aspect ;
   rdfs:range rdfs:Resource .

samm:parameters a mmm:Attribute ;
   rdfs:label "parameters" ;
   rdfs:comment "The parameters defined by an Event." ;
   rdfs:domain samm:Event ;
   rdfs:range rdfs:Resource .

samm:exampleValue a mmm:Attribute ;
   rdfs:label "exampleValue" ;
   rdfs:comment "An exemplary value the Property can take on that helps to understand the intended meaning of the property better. This attribute supports both scalar literal values (e.g., xsd:string or xsd:float), an anonymous described scalar value and value references example values (i.e., references to instances of samm:Value enriched with semantic metadata). The data type of the samm:exampleValue must be convertable to the effective data type of the Property’s Characteristic." ;
   rdfs:domain samm:Property ;
   rdfs:range rdfs:Resource .

samm:extends a mmm:Attribute ;
   rdfs:label "extends" ;
   rdfs:comment "Defines that the target extends the source" ;
   rdfs:domain mmm:Concept ;
   rdfs:range rdfs:Resource .

samm:optional a mmm:Attribute ;
   rdfs:label "optional" ;
   rdfs:comment "Defines whether a Property is optional or not in the context where the Property is being used. The default is false." ;
   rdfs:domain mmm:PropertyUsage ;
   rdfs:range xsd:boolean .

samm:property a mmm:Attribute ;
   rdfs:label "property" ;
   rdfs:comment "Links a Property Usage to an actual Property" ;
   rdfs:domain mmm:PropertyUsage ;
   rdfs:range samm:Property .

samm:notInPayload a mmm:Attribute ;
   rdfs:label "notInPayload" ;
   rdfs:comment "Defines whether a Property is included in the payload of an Aspect. The default is false." ;
   rdfs:domain mmm:PropertyUsage ;
   rdfs:range xsd:boolean .

samm:payloadName a mmm:Attribute ;
   rdfs:label "payloadName" ;
   rdfs:comment "Provides the name of the Property as it will appear in the runtime payload." ;
   rdfs:domain mmm:PropertyUsage ;
   rdfs:range xsd:string .

samm:see a mmm:Attribute ;
   rdfs:label "see" ;
   rdfs:comment "Contains a link to an external taxonomy/ontology." ;
   rdfs:domain mmm:Concept ;
   rdfs:range rdfs:Resource .

samm:commonCode a mmm:Attribute ;
   rdfs:label "commonCode" ;
   rdfs:comment "Normalized short code for a unit." ;
   rdfs:domain samm:Unit ;
   rdfs:range xsd:string .

samm:conversionFactor a mmm:Attribute ;
   rdfs:label "conversionFactor" ;
   rdfs:comment "If the unit is derived from a reference unit, the human readable multiplication factor, e.g., \"10⁻²⁸ m²\"" ;
   rdfs:domain samm:Unit ;
   rdfs:range xsd:string .

samm:numericConversionFactor a mmm:Attribute ;
   rdfs:label "numericConversionFactor" ;
   rdfs:comment "If the unit is derived from a reference unit, the numeric multiplication factor, e.g., \"1.0E-28\"" ;
   rdfs:domain samm:Unit ;
   rdfs:range xsd:double .

samm:quantityKind a mmm:Attribute ;
   rdfs:label "quantityKind" ;
   rdfs:comment "A quantity kind for this unit, for example the unit litre has the quantity kind volume, the unit metre has the quantity kinds length, distance, diameter etc." ;
   rdfs:domain samm:Unit ;
   rdfs:range samm:QuantityKind .

samm:referenceUnit a mmm:Attribute ;
   rdfs:label "referenceUnit" ;
   rdfs:comment "The unit this unit is derived from, e.g., centimetre is derived from metre" ;
   rdfs:domain samm:Unit ;
   rdfs:range samm:Unit .

samm:symbol a mmm:Attribute ;
   rdfs:label "symbol" ;
   rdfs:comment "The unit’s symbol, e.g., for centimetre the symbol is cm" ;
   rdfs:domain samm:Unit ;
   rdfs:range xsd:string .

# Constants
samm:US-ASCII a mmm:Constant .

samm:ISO-8859-1 a mmm:Constant .

samm:UTF-8 a mmm:Constant .

samm:UTF-16 a mmm:Constant .

samm:UTF-16BE a mmm:Constant .

samm:UTF-16LE a mmm:Constant .

# Datatypes
samm:curie a rdfs:Datatype ;
   rdfs:comment "The ·lexical space· of curie is finite-length character sequences which represent a valid curie as defined here https://www.w3.org/TR/2010/NOTE-curie-20101216/#s_schema.";
   rdfs:label "curie" .
